coq/typ_monads.v
@@ -2,18 +2,18 @@ Require Import Snarky.monad.
 
 Module Store.
 
-  Inductive t (F V A : Type) : Type :=
+  Polymorphic Inductive t (F V A : Type) : Type :=
   | Pure : A -> t F V A
   | Free : F -> (V -> t F V A) -> t F V A.
 
   Arguments Pure {F V A} _.
   Arguments Free {F V A} _ _.
 
-  Global Instance store_return F V : Return (t F V) := {
+  Global Polymorphic Instance store_return F V : Return (t F V) := {
     ret A a := Pure a
   }.
 
-  Global Instance store_bind F V : Bind (t F V) := {
+  Global Polymorphic Instance store_bind F V : Bind (t F V) := {
     bind A B t f :=
       (fix bind' t :=
         match t with
@@ -22,7 +22,7 @@ Module Store.
         end) t
   }.
 
-  Global Instance store_map F V : Map (t F V) := {
+  Global Polymorphic Instance store_map F V : Map (t F V) := {
     map A B t f :=
       (fix map' t :=
         match t with
@@ -31,10 +31,26 @@ Module Store.
         end) t
   }.
 
-  Definition store {F V} (x : F) : t F V V :=
+  Module Monad.
+    Section Monad.
+      Context {F V A B : Type}.
+
+      Definition map : t F V A -> (A -> B) -> t F V B := map.
+      Definition bind : t F V A -> (A -> t F V B) -> t F V B := bind.
+      Definition both : t F V A -> t F V B -> t F V (A * B) := both.
+      Definition ret : A -> t F V A := ret.
+      Definition join : t F V (t F V A) -> t F V A := join.
+      Definition ignore_m : t F V A -> t F V unit := ignore_m.
+      Definition all : list (t F V A) -> t F V (list A) := all.
+    End Monad.
+  End Monad.
+
+  Include Monad.
+
+  Polymorphic Definition store {F V} (x : F) : t F V V :=
     Free x (fun v => Pure v).
 
-  Fixpoint run {F V A} (t : t F V A) (f : F -> V) : A :=
+  Polymorphic Fixpoint run {F V A} (t : t F V A) (f : F -> V) : A :=
     match t with
     | Pure x => x
     | Free x k => run (k (f x)) f
@@ -44,18 +60,18 @@ End Store.
 
 Module Read.
 
-  Inductive t (F V A : Type) : Type :=
+  Polymorphic Inductive t (F V A : Type) : Type :=
   | Pure : A -> t F V A
   | Free : V -> (F -> t F V A) -> t F V A.
 
   Arguments Pure {F V A} _.
   Arguments Free {F V A} _ _.
 
-  Global Instance read_return F V : Return (t F V) := {
+  Global Polymorphic Instance read_return F V : Return (t F V) := {
     ret A a := Pure a
   }.
 
-  Global Instance read_bind F V : Bind (t F V) := {
+  Global Polymorphic Instance read_bind F V : Bind (t F V) := {
     bind A B t f :=
       (fix bind' t :=
         match t with
@@ -64,7 +80,7 @@ Module Read.
         end) t
   }.
 
-  Global Instance read_map F V : Map (t F V) := {
+  Global Polymorphic Instance read_map F V : Map (t F V) := {
     map A B t f :=
       (fix map' t :=
         match t with
@@ -73,10 +89,24 @@ Module Read.
         end) t
   }.
 
-  Definition read {F V} (x : V) : t F V F :=
+  Module Monad.
+    Section Monad.
+      Context {F V A B : Type}.
+
+      Definition map : t F V A -> (A -> B) -> t F V B := map.
+      Definition bind : t F V A -> (A -> t F V B) -> t F V B := bind.
+      Definition both : t F V A -> t F V B -> t F V (A * B) := both.
+      Definition ret : A -> t F V A := ret.
+      Definition join : t F V (t F V A) -> t F V A := join.
+      Definition ignore_m : t F V A -> t F V unit := ignore_m.
+      Definition all : list (t F V A) -> t F V (list A) := all.
+    End Monad.
+  End Monad.
+
+  Polymorphic Definition read {F V} (x : V) : t F V F :=
     Free x ret.
 
-  Fixpoint run {F V A} (t : t F V A) (f : V -> F) : A :=
+  Polymorphic Fixpoint run {F V A} (t : t F V A) (f : V -> F) : A :=
     match t with
     | Pure x => x
     | Free x k => run (k (f x)) f
@@ -86,18 +116,18 @@ End Read.
 
 Module Alloc.
 
-  Inductive t (V A : Type) : Type :=
+  Polymorphic Inductive t (V A : Type) : Type :=
   | Pure : A -> t V A
   | Free : (V -> t V A) -> t V A.
 
   Arguments Pure {V A} _.
   Arguments Free {V A} _.
 
-  Global Instance alloc_return V : Return (t V) := {
+  Global Polymorphic Instance alloc_return V : Return (t V) := {
     ret A a := Pure a
   }.
 
-  Global Instance alloc_bind V : Bind (t V) := {
+  Global Polymorphic Instance alloc_bind V : Bind (t V) := {
     bind A B t f :=
       (fix bind' t :=
         match t with
@@ -106,7 +136,7 @@ Module Alloc.
         end) t
   }.
 
-  Global Instance alloc_map V : Map (t V) := {
+  Global Polymorphic Instance alloc_map V : Map (t V) := {
     map A B t f :=
       (fix map' t :=
         match t with
@@ -115,10 +145,24 @@ Module Alloc.
         end) t
   }.
 
-  Definition alloc {V} : t V V :=
+  Module Monad.
+    Section Monad.
+      Context {V A B : Type}.
+
+      Definition map : t V A -> (A -> B) -> t V B := map.
+      Definition bind : t V A -> (A -> t V B) -> t V B := bind.
+      Definition both : t V A -> t V B -> t V (A * B) := both.
+      Definition ret : A -> t V A := ret.
+      Definition join : t V (t V A) -> t V A := join.
+      Definition ignore_m : t V A -> t V unit := ignore_m.
+      Definition all : list (t V A) -> t V (list A) := all.
+    End Monad.
+  End Monad.
+
+  Polymorphic Definition alloc {V} : t V V :=
     Free (fun v => Pure v).
 
-  Fixpoint run {V A} (t : t V A) (f : unit -> V) : A :=
+  Polymorphic Fixpoint run {V A} (t : t V A) (f : unit -> V) : A :=
     match t with
     | Pure x => x
     | Free k => run (k (f tt)) f
